\chapter{Holes Analysis Proofs}
\label{appendix:holes}

To show the bound on the expected number of holes, we present some claims. 

In Section~\ref{sec:holes-analysis} we show in Equation~\ref{eq:pi-i-j} that 
\begin{align*}
\pi_{i,j} \leq \left(\frac{1}{2}\right)^{jb + 2i +1} {{jb+2i} \choose i}.
\end{align*}
Consider the following functions:
\begin{align*}
f_1(i) &\triangleq \left(\frac{1}{2}\right)^{jb + 2i +1} {{jb+2i} \choose i}. \\
f_2(i) &\triangleq \frac{1}{4} \cdot \frac{(jb+2i+2)(jb+2i+1)}{(jb+i+1)(i+1)}. \\
f_3(j) &\triangleq \frac{1}{4} \cdot \frac{(jb+2b)(jb+2b-1)}{(jb+b)b}.
\end{align*}

\begin{claim}\label{claim:f-2-dec}
$f_2(i)$ is monotonically decreasing for $0 \leq i \leq b-1$ and for $j,b>2 \in \mathds{N}$. 
\end{claim}

\begin{proof}
\begin{align*}
    f_2(i+1) &= \frac{1}{4} \cdot \frac{(jb+2i+4)(jb+2i+3)}{(jb+i+2)(i+2)}.
\end{align*}
We show that $\frac{f_2(i+1)}{f_2(i)} \leq 1$ for $0 \leq i \leq b-2$.
\begin{align*}
    \frac{f_2(i+1)}{f_2(i)} &= \frac{(jb+2i+4)}{(jb+2i+2)} \cdot \frac{(jb+2i+3)}{(jb+2i+1)} \cdot \frac{(jb+i+1)}{(jb+i+2)} \cdot \frac{(i+1)}{(i+2)} 
    % \\
    % &\leq \underbrace{\frac{(jb+2i)}{(jb+2i+2)}}_{\leq 1} \cdot \underbrace{\frac{(jb+2i)}{(jb+2i+1)}}_{\leq 1} \cdot \underbrace{\frac{(jb+i+1)}{(jb+i+2)}}_{\leq 1} \cdot \underbrace{\frac{(i+1)}{(i+2)}}_{\leq 1} 
    \leq 1
\end{align*}
\end{proof}

\begin{claim}\label{claim:f-3-inc}
$f_3(j)$ is monotonically increasing for $j,b>2 \in \mathds{N}$. 
\end{claim}

\begin{proof}
\begin{align*}
    f_3(j+1) = \frac{1}{4} \cdot \frac{(jb+3b)(jb+3b-1)}{(jb+2b)b}.
\end{align*}
We show that $\frac{f_3(j+1)}{f_3(j)} \geq 1$ for $j,b>2 \in \mathds{N}$
\begin{align*}
    \frac{f_3(j+1)}{f_3(j)} &= \underbrace{\frac{(jb+3b)}{(jb+2b)}}_{\geq 1} \cdot \underbrace{\frac{(jb+3b-1)}{(jb+2b-1)}}_{\geq 1} \cdot \frac{(jb+b)}{(jb+2b)} \\
    &\geq \frac{(jb+b)}{(jb+2b)} \geq \frac{(jb+2b)}{(jb+2b)}
    \geq 1 
\end{align*}
\end{proof}


\begin{claim}\label{claim:holes-pi-mono}
$f_1(i)$ is monotonically increasing for $i \in \{0,1,\dots,b-1\}$ and for $j,b \in \mathds{N}$. 
\end{claim}

\begin{proof}
For $b=1$, $i \in {0}$ and the claim is immediate.\\
For $b=2$, $i \in {0,1}$ thus,
\begin{align*}
    f_1(0) &= \left(\frac{1}{2}\right)^{2j+1} \\
    f_1(1) &= \left(\frac{1}{2}\right)^{2j+3} {{2j+2} \choose 1} \\
            &= \left(\frac{1}{2}\right)^{2j+1} \cdot \left(\frac{1}{2}\right)^{2} \cdot (2j+2)\\
            &= f_1(0) \cdot \frac{2j+2}{4} \geq f_1(0) \cdot \frac{2+2}{4} = f_1(0).
\end{align*}
For $b>2$, we show that $f_1(i+1)\geq f_1(i)$ for all $0 \leq i \leq b-1$ and for $j,b \in \mathds{N}$

\begin{align*}
    f_1(i) &= \left(\frac{1}{2}\right)^{jb + 2i +1} {{jb+2i} \choose {i}} \\
    f_1(i+1) &= \left(\frac{1}{2}\right)^{jb + 2i +3} {{jb+2i+2} \choose {i+1}} \\
    &= \left(\frac{1}{2}\right)^{jb + 2i +3} \cdot \frac{(jb+2i+2)!}{(jb+i+1)!\cdot(i+1)!} \\
    &= f_1(i) \cdot \frac{1}{4} \cdot \frac{(jb+2i+2)(jb+2i+1)}{(jb+i+1)(i+1)}
\end{align*}

Claim~\ref{claim:f-2-dec} shows that $f_2(i) = \frac{1}{4} \cdot \frac{(jb+2i+2)(jb+2i+1)}{(jb+i+1)(i+1)} $ is monotonically decreasing for $0\leq{i}\leq{b-1}$. 
Denote by $f_3(j)$ to be $f_2(b-1)$,
\begin{align}
    f_3(j) &\triangleq \frac{1}{4} \cdot \frac{(jb+2b)(jb+2b-1)}{(jb+b)b}
\end{align}

Claim~\ref{claim:f-3-inc} shows that $f_3(j)$ is monotonically increasing. 
\begin{align*}
    f_3(1) &= \frac{1}{4} \cdot \frac{(3b)(3b-1)}{2b^2} = \frac{9b-3}{8b} \underbrace{=}_{b\geq 3} \frac{9b-b}{8b} \geq 1
\end{align*}

Therefore, $f_3(j) \geq 1$ for all $j\geq1$.
With this, we have shown that 
\begin{align*}
f_1(i+1) = f_1(i) \cdot \frac{1}{4} \cdot \frac{(jb+2i+2)(jb+2i+1)}{(jb+i+1)(i+1)} \geq f_1(i)
\end{align*}

\end{proof}

\begin{claim}\label{claim:g-1}
$g_1(b) \triangleq \frac{3b-1}{b}$ bounded by 3.
\end{claim}

\begin{proof}
\begin{align*}
    g_1(b) = \frac{3b-1}{b} < \frac{3b}{b} < 3
\end{align*}
\end{proof}

\begin{claim}\label{claim:g-2}
$g_2(b) \triangleq \frac{3b+1}{2b+1}$ bounded by 1.5.
\end{claim}

\begin{proof}
\begin{align*}
    g_2(b) = \frac{3b+1}{2b+1} = \frac{(2b+1) + b }{2b+1} = 1 + \frac{b}{2b+1} < 1 + \frac{b}{2b} < 1.5
\end{align*}
\end{proof}

\begin{claim}\label{claim:g-3}
$g_3(b) \triangleq \frac{(b+1)^2}{b^2}$ is monotonically decreasing and for $b=12$, $g_3(b)= \left(\frac{13}{12}\right)^2$ 
\end{claim}

\begin{proof}
The proof is immediate. 
\end{proof}

\begin{claim} \label{claim:E-H-j-help}
$\left(\frac{1}{2}\right)^{b-1} \cdot {{jb+3b-2} \choose {b-1}} \leq {{jb+2b-2} \choose {b-1}}$ for all $b\in \mathds{N}$ and $j\geq1, j\in \mathds{N}$. 
\end{claim}

\begin{proof}
\begin{align*}
    & \left(\frac{1}{2}\right)^{b-1} \cdot {{jb+3b-2} \choose {b-1}} = \\
    & \left(\frac{1}{2}\right)^{b-1} \cdot \frac{(jb+3b-2)!}{(b-1)!(jb+2b-1)!} =\\
    & \left(\frac{1}{2}\right)^{b-1} \cdot \frac{(jb+2b-2+b)!}{(b-1)!(jb+b-1+b)!} =\\
    & \left(\frac{1}{2}\right)^{b-1} \cdot \frac{(jb+2b-2)!}{(b-1)!(jb+b-1)!} \cdot 
    \frac{(jb+2b-2+1)\cdots(jb+2b-2+b)}{(jb+b-1+1)\cdots(jb+b-1+b)} =\\
    & \left(\frac{1}{2}\right)^{b-1} \cdot {{jb+2b-2} \choose {b-1}} \cdot \prod_{t=1}^b \frac{jb+2b-2+t}{jb+b-1+t} =\\
    & {{jb+2b-2} \choose {b-1}} \cdot \prod_{t=1}^b \frac{jb+2b-2+t}{2(jb+b-1+t)} =\\
    & {{jb+2b-2} \choose {b-1}} \cdot \underbrace{\prod_{t=1}^b \frac{jb+2b-2+t}{(jb+2b-2+t)+jb+t}}_{\leq1} \leq {{jb+2b-2} \choose {b-1}}
\end{align*}
for all $b,j\in \mathds{N}$ such that $j\geq1$.
\end{proof}